src/RsUpRed.v
@@ -42,13 +42,10 @@ Section RsUpReduction.
             oorq@[downRq] = Some orqid /\
             DownLockedInv dtr st1.(bst_orqs) st1.(bst_msgs) oidx orqid).
   Proof.
-    intros; destruct Hrrs as [? [? ?]].
-
+    intros; destruct Hrrs as [? [? [_ ?]]].
     pose proof (footprints_ok H3 H0).
-    pose proof (downLockInv_ok H3 H2 H0).
-
+    pose proof (downLockInv_ok H3 H2 H4 H0).
     red in H; dest.
-
     inv_step.
     good_rqrs_rule_get rule.
     good_rqrs_rule_cases rule.
@@ -353,8 +350,8 @@ Section RsUpReduction.
           step_m sys st1 (RlblInt oidx ridx rins routs) st2 ->
           DisjList (idsOf rsUps) (idsOf rins).
   Proof.
-    destruct Hrrs as [? [? ?]]; intros.
-    pose proof (downLockInv_ok H0 H H7).
+    destruct Hrrs as [? [? [_ ?]]]; intros.
+    pose proof (downLockInv_ok H0 H H1 H7).
     good_locking_get objTo; clear H10.
 
     apply (DisjList_false_spec eq_nat_dec); intros rsUp Hin1 Hin2.
@@ -400,7 +397,7 @@ Section RsUpReduction.
           step_m sys st1 (RlblInt oidx ridx rins routs) st2 ->
           DisjList routs rsUps.
   Proof.
-    destruct Hrrs as [? [? ?]].
+    destruct Hrrs as [? [? [_ ?]]].
     intros.
     eapply rsUp_lbl_rins_ids_disj in H5; eauto; clear H4.
 
@@ -410,7 +407,7 @@ Section RsUpReduction.
     }
 
     inv_step; simpl in *.
-    pose proof (downLockInv_ok H0 H H4).
+    pose proof (downLockInv_ok H0 H H1 H4).
     good_locking_get objTo; clear H9.
     
     apply (DisjList_false_spec (id_dec msg_dec)); intros rsUp Hin1 Hin2.
